Fix names of ind principles, add EJCP'06 slides

proof/Russell/RussellMinus/Types.v
@@ -7,49 +7,78 @@ Require Import Env.
 Set Implicit Arguments.
 
 Implicit Types i k m n p : nat.
-Implicit Type t : sort.
-Implicit Types A B M N T u v : term.
+Implicit Types A B M N T t u v : term.
 
 Reserved Notation "G ||- T : s" (at level 70, T, s at next level).
 
 Inductive type : Set :=
-  | in_set : type
-  | in_prop : type
-  | star : type
-  | box : type.
+  | orig_set : type
+  | orig_prop : type
+  | kind_prop : type
+  | kind_set : type
+  | triangle_set : type
+  | triangle_prop : type.
 
-Definition interp (s : sort) : type :=
-  match s with
-  | prop => in_prop
-  | set => in_set
-  | kind => star
-  end.
+Definition is_orig (t : type) := t <> triangle_set /\ t <> triangle_prop.
 
-Definition sum_sort' s1 s2 s3 :=
-  (s1 = in_set /\ s2 = in_set /\ s3 = in_set) \/
-  (s1 = star /\ s2 = in_set /\ s3 = star) \/
-  (s1 = in_set /\ s2 = star /\ s3 = star) \/
-  (s1 = in_prop /\ s2 = in_prop /\ s3 = in_prop).
+Definition interp (t : type) : is_orig t -> type.
+induction t ; intros.
+exact triangle_set.
+exact triangle_prop.
+exact orig_prop.
+exact orig_set.
+unfold is_orig in H ; simpl in H.
+intuition.
+unfold is_orig in H ; simpl in H.
+intuition.
+Defined.
+
+Lemma is_orig_set : is_orig orig_set.
+Proof.
+  unfold is_orig ; simpl ; auto ; intuition ; discriminate.
+Qed.
+
+Lemma is_orig_prop : is_orig orig_prop.
+Proof.
+  unfold is_orig ; simpl ; auto ; intuition ; discriminate.
+Qed.
+
+Lemma is_orig_kind_prop : is_orig kind_prop.
+Proof.
+  unfold is_orig ; simpl ; auto ; intuition ; discriminate.
+Qed.
+
+Lemma is_orig_kind_set : is_orig kind_set.
+Proof.
+  unfold is_orig ; simpl ; auto ; intuition ; discriminate.
+Qed.
+
+Definition sum_sort s1 s2 s3 :=
+  (s1 = orig_set /\ s2 = orig_set /\ s3 = orig_set) \/
+  (s1 = kind_set /\ s2 = orig_set /\ s3 = kind_set) \/
+  (s1 = orig_set /\ s2 = kind_set /\ s3 = kind_set) \/
+  (s1 = orig_set /\ s2 = kind_prop /\ s3 = kind_prop) \/
+  (s1 = orig_prop /\ s2 = orig_prop /\ s3 = orig_prop).
+
 
 Inductive wf_minus : env -> Prop :=
   | wf_nil : wf_minus nil
-  | wf_var : forall e T s, e ||- T : s -> wf_minus (T :: e)
+  | wf_var_set : forall e T s, e ||- T : s -> is_orig s -> wf_minus (T :: e)
 
 with typ_minus : env -> term -> type -> Prop :=
-  | type_minus_prop : forall e, wf_minus e -> e ||- (Srt prop) : star
-  | type_minus_set : forall e, wf_minus e -> e ||- (Srt set) : star
+  | type_minus_prop : forall e, wf_minus e -> e ||- (Srt prop) : kind_prop
+  | type_minus_set : forall e, wf_minus e -> e ||- (Srt set) : kind_set
 
   | type_minus_var : (* start *)
   forall e, wf_minus e -> forall n T, item_lift T e n ->
-  forall s, e ||- T : s -> e ||- (Ref n) : s
+  forall s, e ||- T : s -> forall H : is_orig s, e ||- (Ref n) : interp H
 
   | type_minus_abs :
-      forall e T s1,
-      e ||- T : s1 ->
-      forall M (U : term) s2,
-      (T :: e) ||- U : s2 ->
-      (T :: e) ||- M : s2 -> 
-      e ||- (Abs T M) : s2
+    forall e T B s, e ||- Prod T B : s ->
+    forall H : is_orig s, 
+    forall M, (T :: e) ||- M : interp H -> 
+    e ||- (Abs T M) : interp H
+
   | type_minus_app :
       forall e v s1, e ||- v : s1 ->
       forall u s, e ||- u : s -> 
@@ -60,7 +89,7 @@ with typ_minus : env -> term -> type -> Prop :=
     forall u su, e ||- u : su ->
     forall V s2, (U :: e) ||- V : s2 ->
     forall v, e ||- v : s2 -> 
-    forall s3, sum_sort' s1 s2 s3 ->
+    forall s3, sum_sort s1 s2 s3 ->
     e ||- (Pair (Sum U V) u v) : s3
 
   | type_minus_prod :
@@ -68,6 +97,7 @@ with typ_minus : env -> term -> type -> Prop :=
       e ||- T : s1 ->
       forall (U : term) s2,
       (T :: e) ||- U : s2 -> 
+      is_orig s1 -> is_orig s2 ->
       e ||- (Prod T U) : s2
 
   | type_minus_sum :
@@ -75,13 +105,13 @@ with typ_minus : env -> term -> type -> Prop :=
       e ||- T : s1 ->
       forall (U : term) s2,
       (T :: e) ||- U : s2 -> 
-      forall s3, sum_sort' s1 s2 s3 ->
+      forall s3, sum_sort s1 s2 s3 ->
       e ||- (Sum T U) : s3
 
   | type_minus_subset : 
-      forall e T, e ||- T : in_set ->
-      forall (U : term), (T :: e) ||- U : in_prop -> 
-      e ||- (Subset T U) : in_set
+      forall e T, e ||- T : orig_set ->
+      forall (U : term), (T :: e) ||- U : orig_prop -> 
+      e ||- (Subset T U) : orig_set
 
   | type_minus_pi1 :
       forall e (t : term) s, e ||- t : s -> 
@@ -104,20 +134,99 @@ where "G ||- T : U" :=  (typ_minus G T U).
 Hint Resolve type_minus_pi1 type_minus_pi2 type_minus_pair type_minus_prop type_minus_set type_minus_var: coc.
 
 Require Import CCPD.Types.
+Require Import CCPD.Thinning.
+Require Import CCPD.Generation.
 
 Lemma soundness : forall G (t : term) T, G |- t : T ->
-  (forall s, G |- T : (Srt s) -> is_prop s -> G ||- t : (interp s)).
+ ((G |- T : (Srt set) -> G ||- t : triangle_set) /\
+ (G |- T : (Srt prop) -> G ||- t : triangle_prop) /\
+ (G |- T : Srt kind -> G ||- t : orig_set \/ G ||- t : orig_prop) /\
+ (T = Srt kind -> G ||- t : kind_set \/ G ||- t : kind_prop)).
 Proof.
-  induction 1 ; simpl ; intros.
+  induction 1 using typ_wf_mut with
+  (P := fun G t (T : term) => fun H0 : G |- t : T =>
+ ((G |- T : (Srt set) -> G ||- t : triangle_set) /\
+ (G |- T : (Srt prop) -> G ||- t : triangle_prop) /\
+ (G |- T : Srt kind -> G ||- t : orig_set \/ G ||- t : orig_prop) /\
+ (T = Srt kind -> G ||- t : kind_set \/ G ||- t : kind_prop)))
+  (P0 := fun G => fun H : wf G => 
+  wf_minus G /\
+  forall T G n, item_lift T G n -> 
+  (G |- T : Srt set -> G ||- T : orig_set) /\
+  (G |- T : Srt prop -> G ||- T : orig_prop) /\
+  (G |- T : Srt kind -> G ||- T : kind_set \/ G ||- T : kind_prop))
+ ; simpl ; intros.
+  
+  intuition ; intros.
+  elim (typ_not_kind H1) ; auto.
+  elim (typ_not_kind H1) ; auto.
 
+  intuition ; intros.
+  elim (typ_not_kind H1) ; auto.
+
+  intuition ; intros.
+  elim (typ_not_kind H1) ; auto.
+  elim (typ_not_kind H1) ; auto.
+  elim (typ_not_kind H1) ; auto.
+
+  split ; intros.
+  destruct IHtyp.
+  destruct (H1 T e n i).
+  pose (H2 H).
+  pose (type_minus_var H0 i t (is_orig_set)).
+  simpl in t0 ; assumption.
+
+  split ; intros.
+  destruct IHtyp.
+  destruct (H1 T e n i).
+  destruct H3.
+  pose (H3 H).
+  pose (type_minus_var H0 i t (is_orig_prop)).
+  simpl in t0 ; assumption.
+
+  split ; intros.
+  destruct IHtyp.
+  destruct (H1 T e n i).
+  destruct H3.
+  pose (H4 H).
+  destruct o.
+  left.
+  pose (type_minus_var H0 i H5 (is_orig_kind_set)).
+  simpl in t ; assumption.
+
+  right.
+  pose (type_minus_var H0 i H5 (is_orig_kind_prop)).
+  simpl in t ; assumption.
+
+  destruct (wf_sort_lift w i).
+  rewrite H in H0.
   elim (typ_not_kind H0) ; auto.
 
-  elim (typ_not_kind H0) ; auto.
 
-  induction s ; simpl ; auto with coc.
-  unfold is_prop in H2 ; intuition ; try discriminate.
-  apply type_minus_var with T ; auto with coc.
-  unfold is_prop in H2 ; intuition ; try discriminate.
+  split ; intros.
+  intuition.
+
+  pose (generation_prod2 H2).
+  destruct a.
+  pose (H7 H16).
+  destruct (type_sorted H).
+  cut (e ||- Prod T U : orig_set) ; intros.
+  assert(triangle_set = interp is_orig_set).
+  simpl ; auto.
+  rewrite H19.
+  apply (@type_minus_abs e T U orig_set H18).
+  simpl ; auto.
+  pose (H13 H17).
+  destruct o.
+  eapply type_minus_prod with kind_set ; auto.
+  
+ with orig_set.
+  with kind_set ; auto with coc.
+
+
+.
+
+  unfold is_prop in H0 ; intuition ; try discriminate.
 
 
 
